fstar/treedem/MLS.TreeDEM.Welcome.fst
@@ -14,248 +14,6 @@ open MLS.Result
 
 #set-options "--fuel 0 --ifuel 0"
 
-type group_context (bytes:Type0) {|bytes_like bytes|} = {
-  version: protocol_version_nt;
-  cipher_suite: cipher_suite_nt;
-  group_id: bytes;
-  epoch: nat;
-  tree_hash: bytes;
-  confirmed_transcript_hash: bytes;
-  extensions: list (extension_nt bytes);
-}
-
-type welcome_group_info (bytes:Type0) {|bytes_like bytes|} = {
-  group_context: group_context bytes;
-  extensions: bytes;
-  confirmation_tag: bytes;
-  signer: nat;
-  signature: bytes;
-}
-
-type group_secrets (bytes:Type0) {|bytes_like bytes|} = {
-  joiner_secret: bytes;
-  path_secret: option bytes;
-  psks: list (pre_shared_key_nt bytes);
-}
-
-//TODO: move in Crypto? (copy-pasted from TreeKEM)
-type hpke_ciphertext (bytes:Type0) {|bytes_like bytes|} = {
-  kem_output: bytes;
-  ciphertext: bytes;
-}
-
-type encrypted_group_secrets (bytes:Type0) {|bytes_like bytes|} = {
-  new_member: key_package_ref_nt bytes;
-  enc_group_secrets: hpke_ciphertext bytes
-}
-
-type welcome (bytes:Type0) {|bytes_like bytes|} = {
-  //version ?
-  //cipher_suite ?
-  secrets: list (encrypted_group_secrets bytes);
-  encrypted_group_info: bytes;
-}
-
-(*** From / to network ***)
-
-val network_to_group_context:
-  #bytes:Type0 -> {|bytes_like bytes|} ->
-  group_context_nt bytes ->
-  group_context bytes
-let network_to_group_context #bytes #bl gc =
-  {
-    version = gc.version;
-    cipher_suite = gc.cipher_suite;
-    group_id = gc.group_id;
-    epoch = gc.epoch;
-    tree_hash = gc.tree_hash;
-    confirmed_transcript_hash = gc.confirmed_transcript_hash;
-    extensions = gc.extensions;
-  }
-
-val network_to_welcome_group_info:
-  #bytes:Type0 -> {|bytes_like bytes|} ->
-  group_info_nt bytes ->
-  welcome_group_info bytes
-let network_to_welcome_group_info #bytes #bl gi =
-  {
-    group_context = network_to_group_context gi.tbs.group_context;
-    extensions = gi.tbs.extensions;
-    confirmation_tag = gi.tbs.confirmation_tag;
-    signer = gi.tbs.signer;
-    signature = gi.signature;
-  }
-
-val group_context_to_network:
-  #bytes:Type0 -> {|crypto_bytes bytes|} ->
-  group_context bytes ->
-  result (group_context_nt bytes)
-let group_context_to_network #bytes #bl gc =
-  if not (length gc.group_id < pow2 30) then
-    internal_failure "group_context_to_network: group_id too long"
-  else if not (gc.epoch < pow2 64) then
-    internal_failure "group_context_to_network: epoch too big"
-  else if not (length gc.tree_hash < pow2 30) then
-    internal_failure "group_context_to_network: tree_hash too long"
-  else if not (length gc.confirmed_transcript_hash < pow2 30) then
-    internal_failure "group_context_to_network: confirmed_transcript_hash too long"
-  else if not (bytes_length ps_extension_nt gc.extensions < pow2 30) then
-    internal_failure "group_context_to_network: extensions too long"
-  else
-    return ({
-      version = gc.version;
-      cipher_suite = gc.cipher_suite;
-      group_id = gc.group_id;
-      epoch = gc.epoch;
-      tree_hash = gc.tree_hash;
-      confirmed_transcript_hash = gc.confirmed_transcript_hash;
-      extensions = gc.extensions;
-    } <: group_context_nt bytes)
-
-
-val welcome_group_info_to_network:
-  #bytes:Type0 -> {|crypto_bytes bytes|} ->
-  welcome_group_info bytes ->
-  result (group_info_nt bytes)
-let welcome_group_info_to_network #bytes #bl gi =
-  if not (length gi.extensions < pow2 30) then
-    internal_failure "welcome_group_info_to_network: other_extensions too long"
-  else if not (length gi.confirmation_tag < pow2 30) then
-    internal_failure "welcome_group_info_to_network: confirmation_tag too long"
-  else if not (gi.signer < pow2 32) then
-    internal_failure "welcome_group_info_to_network: signer is too big"
-  else if not (length gi.signature < pow2 30) then
-    internal_failure "welcome_group_info_to_network: signature_id too long"
-  else (
-    let? group_context = group_context_to_network gi.group_context in
-    return ({
-      tbs = {
-        group_context;
-        extensions = gi.extensions;
-        confirmation_tag = gi.confirmation_tag;
-        signer = gi.signer;
-      };
-      signature = gi.signature;
-    } <: group_info_nt bytes)
-  )
-
-val network_to_group_secrets:
-  #bytes:Type0 -> {|bytes_like bytes|} ->
-  group_secrets_nt bytes ->
-  result (group_secrets bytes)
-let network_to_group_secrets #bytes #bl gs =
-  return ({
-    joiner_secret = gs.joiner_secret;
-    path_secret = (
-      match gs.path_secret with
-      | None -> None
-      | Some p -> Some p.path_secret
-    );
-    psks = gs.psks;
-  })
-
-val group_secrets_to_network:
-  #bytes:Type0 -> {|bytes_like bytes|} ->
-  group_secrets bytes ->
-  result (group_secrets_nt bytes)
-let group_secrets_to_network #bytes #bl gs =
-  let? path_secret = (
-    match gs.path_secret with
-    | None -> return None
-    | Some p -> (
-      if not (length p < pow2 30) then
-        internal_failure ""
-      else
-        return (Some ({ path_secret = p } <: path_secret_nt bytes))
-    )
-  ) in
-  if not (length gs.joiner_secret < pow2 30) then
-    internal_failure "group_secrets_to_network: joiner_secret too long"
-  else if not (bytes_length ps_pre_shared_key_nt gs.psks < pow2 30) then
-    internal_failure "group_secrets_to_network: psks too long"
-  else (
-    return ({
-      joiner_secret = gs.joiner_secret;
-      path_secret = path_secret;
-      psks = gs.psks;
-    } <: group_secrets_nt bytes)
-  )
-
-val network_to_hpke_ciphertext:
-  #bytes:Type0 -> {|bytes_like bytes|} ->
-  hpke_ciphertext_nt bytes ->
-  hpke_ciphertext bytes
-let network_to_hpke_ciphertext x =
-  ({
-    kem_output = x.kem_output;
-    ciphertext = x.ciphertext;
-  })
-
-val hpke_ciphertext_to_network:
-  #bytes:Type0 -> {|bytes_like bytes|} ->
-  hpke_ciphertext bytes ->
-  result (hpke_ciphertext_nt bytes)
-let hpke_ciphertext_to_network #bytes #bl x =
-  if not (length x.kem_output < pow2 30) then
-    internal_failure "hpke_ciphertext_to_network: kem_output too long"
-  else if not (length x.ciphertext < pow2 30) then
-    internal_failure "hpke_ciphertext_to_network: ciphertext too long"
-  else
-    return ({
-      kem_output = x.kem_output;
-      ciphertext = x.ciphertext
-    } <: hpke_ciphertext_nt bytes)
-
-val network_to_encrypted_group_secrets:
-  #bytes:Type0 -> {|bytes_like bytes|} ->
-  encrypted_group_secrets_nt bytes ->
-  encrypted_group_secrets bytes
-let network_to_encrypted_group_secrets #bytes #bl egs =
-  ({
-    new_member = egs.new_member;
-    enc_group_secrets = network_to_hpke_ciphertext egs.encrypted_group_secrets;
-  })
-
-val encrypted_group_secrets_to_network:
-  #bytes:Type0 -> {|bytes_like bytes|} ->
-  encrypted_group_secrets bytes ->
-  result (encrypted_group_secrets_nt bytes)
-let encrypted_group_secrets_to_network #bytes #bl egs =
-  let? encrypted_group_secrets = hpke_ciphertext_to_network egs.enc_group_secrets in
-  return ({
-    new_member = egs.new_member;
-    encrypted_group_secrets = encrypted_group_secrets;
-  } <: encrypted_group_secrets_nt bytes)
-
-val network_to_welcome:
-  #bytes:Type0 -> {|bytes_like bytes|} ->
-  welcome_nt bytes ->
-  welcome bytes
-let network_to_welcome w =
-  {
-    secrets = List.Tot.map network_to_encrypted_group_secrets w.secrets;
-    encrypted_group_info = w.encrypted_group_info;
-  }
-
-val welcome_to_network:
-  #bytes:Type0 -> {|crypto_bytes bytes|} ->
-  welcome bytes ->
-  result (welcome_nt bytes)
-let welcome_to_network #bytes #cb w =
-  let? secrets = mapM encrypted_group_secrets_to_network w.secrets in
-  let cipher_suite = available_ciphersuite_to_network (ciphersuite #bytes) in
-  if not (length w.encrypted_group_info < pow2 30) then
-    internal_failure "welcome_to_network: encrypted_group_info too long"
-  else if not (bytes_length ps_encrypted_group_secrets_nt secrets < pow2 30) then
-    internal_failure "welcome_to_network: secrets too long"
-  else (
-    return ({
-      cipher_suite = cipher_suite;
-      secrets = secrets;
-      encrypted_group_info = w.encrypted_group_info;
-    } <: welcome_nt bytes)
-  )
-
 (*** Utility functions ***)
 
 val bytes_to_kem_output:
@@ -287,37 +45,37 @@ let welcome_secret_to_nonce #bytes #cb welcome_secret =
 #push-options "--ifuel 1"
 val find_my_encrypted_group_secret:
   #bytes:Type0 -> {|crypto_bytes bytes|} ->
-  (bytes -> option (hpke_private_key bytes)) -> list (encrypted_group_secrets bytes) ->
-  option (hpke_private_key bytes & hpke_ciphertext bytes)
+  (bytes -> option (hpke_private_key bytes)) -> list (encrypted_group_secrets_nt bytes) ->
+  option (hpke_private_key bytes & hpke_ciphertext_nt bytes)
 let rec find_my_encrypted_group_secret #bytes #cb kp_ref_to_hpke_sk l =
   match l with
   | [] -> None
   | h::t -> (
     match kp_ref_to_hpke_sk h.new_member with
-    | Some sk -> Some (sk, h.enc_group_secrets)
+    | Some sk -> Some (sk, h.encrypted_group_secrets)
     | None -> find_my_encrypted_group_secret kp_ref_to_hpke_sk t
   )
 #pop-options
 
 val decrypt_welcome:
   #bytes:Type0 -> {|crypto_bytes bytes|} ->
-  welcome bytes -> (bytes -> option (hpke_private_key bytes)) -> option (l:nat & treesync bytes tkt l 0) ->
-  result (welcome_group_info bytes & group_secrets bytes)
+  welcome_nt bytes -> (bytes -> option (hpke_private_key bytes)) -> option (l:nat & treesync bytes tkt l 0) ->
+  result (group_info_nt bytes & group_secrets_nt bytes)
 let decrypt_welcome #bytes #cb w kp_ref_to_hpke_sk opt_tree =
   let? group_secrets = (
     let? (my_hpke_sk, my_hpke_ciphertext) = from_option "decrypt_welcome: can't find my encrypted secret" (find_my_encrypted_group_secret kp_ref_to_hpke_sk w.secrets) in
     let? kem_output = bytes_to_kem_output my_hpke_ciphertext.kem_output in
     let? group_secrets_bytes = decrypt_with_label my_hpke_sk "Welcome" w.encrypted_group_info kem_output my_hpke_ciphertext.ciphertext in
     let? group_secrets_network = from_option "decrypt_welcome: malformed group secrets" (parse (group_secrets_nt bytes) group_secrets_bytes) in
-    network_to_group_secrets group_secrets_network
+    return group_secrets_network
   ) in
   let? group_info = (
-    let? welcome_secret = secret_joiner_to_welcome group_secrets.joiner_secret None (*TODO psk*) in
+    let? welcome_secret = secret_joiner_to_welcome #bytes group_secrets.joiner_secret None (*TODO psk*) in
     let? welcome_key = welcome_secret_to_key #bytes welcome_secret in
     let? welcome_nonce = welcome_secret_to_nonce welcome_secret in
     let? group_info_bytes = aead_decrypt welcome_key welcome_nonce empty w.encrypted_group_info in
     let? group_info_network = from_option "decrypt_welcome: malformed group info" (parse (group_info_nt bytes) group_info_bytes) in
-    return (network_to_welcome_group_info group_info_network)
+    return (group_info_network)
   ) in
   //TODO: integrity check, this is where `opt_tree` will be useful
   return (group_info, group_secrets)
@@ -326,23 +84,30 @@ let decrypt_welcome #bytes #cb w kp_ref_to_hpke_sk opt_tree =
 
 val encrypt_one_group_secrets:
   #bytes:Type0 -> {|crypto_bytes bytes|} ->
-  key_package_nt bytes tkt -> bytes -> group_secrets bytes -> lbytes bytes (hpke_private_key_length #bytes) ->
-  result (encrypted_group_secrets bytes)
+  key_package_nt bytes tkt -> bytes -> group_secrets_nt bytes -> lbytes bytes (hpke_private_key_length #bytes) ->
+  result (encrypted_group_secrets_nt bytes)
 let encrypt_one_group_secrets #bytes #cb kp encrypted_group_info gs rand =
   let? kp_ref = compute_key_package_ref kp in
-  let? gs_network = group_secrets_to_network gs in
-  let gs_bytes = serialize #bytes (group_secrets_nt bytes) gs_network in
-  let? leaf_hpke_pk = (
+  let gs_bytes = serialize #bytes (group_secrets_nt bytes) gs in
+  let? leaf_hpke_pk: hpke_public_key bytes = (
     let leaf_hpke_pk = kp.tbs.init_key in
     if not (length (leaf_hpke_pk <: bytes) = hpke_public_key_length #bytes) then
       internal_failure "encrypt_one_group_secrets: public key has wrong size"
     else
-      return (leaf_hpke_pk <: hpke_public_key bytes)
+      return leaf_hpke_pk
   ) in
-  let? (kem_output, ciphertext) = encrypt_with_label leaf_hpke_pk "Welcome" encrypted_group_info gs_bytes rand in
+  let? (kem_output, ciphertext) = (
+    let? (kem_output, ciphertext) = encrypt_with_label leaf_hpke_pk "Welcome" encrypted_group_info gs_bytes rand in
+    if not (length #bytes kem_output < pow2 30) then
+      error "encrypt_one_group_secrets: kem_output too long"
+    else if not (length #bytes ciphertext < pow2 30) then
+      error "encrypt_one_group_secrets: ciphertext too long"
+    else
+      return ((kem_output <: mls_bytes bytes), (ciphertext <: mls_bytes bytes))
+  ) in
   return ({
     new_member = kp_ref;
-    enc_group_secrets = {
+    encrypted_group_secrets = {
       kem_output = kem_output;
       ciphertext = ciphertext;
     }
@@ -351,7 +116,7 @@ let encrypt_one_group_secrets #bytes #cb kp encrypted_group_info gs rand =
 #push-options "--fuel 1 --ifuel 1"
 val encrypt_welcome_entropy_length:
   #bytes:Type0 -> {|crypto_bytes bytes|} ->
-  list (key_package_nt bytes tkt & option bytes) ->
+  list (key_package_nt bytes tkt & option (mls_bytes bytes)) ->
   list nat
 let rec encrypt_welcome_entropy_length #bytes #cb leaf_packages =
   match leaf_packages with
@@ -362,13 +127,18 @@ let rec encrypt_welcome_entropy_length #bytes #cb leaf_packages =
 #push-options "--fuel 1 --ifuel 1 --z3rlimit 50"
 val encrypt_group_secrets:
   #bytes:Type0 -> {|crypto_bytes bytes|} ->
-  bytes -> bytes -> key_packages:list (key_package_nt bytes tkt & option bytes) -> list (pre_shared_key_nt bytes) -> randomness bytes (encrypt_welcome_entropy_length key_packages) ->
-  result (list (encrypted_group_secrets bytes))
+  bytes -> mls_bytes bytes -> key_packages:list (key_package_nt bytes tkt & option (mls_bytes bytes)) -> mls_list bytes ps_pre_shared_key_nt -> randomness bytes (encrypt_welcome_entropy_length key_packages) ->
+  result (list (encrypted_group_secrets_nt bytes))
 let rec encrypt_group_secrets #bytes #cb encrypted_group_info joiner_secret key_packages psks rand =
   match key_packages with
   | [] -> return []
   | (kp, path_secret)::tail -> (
     let (cur_rand, rand_next) = dest_randomness rand in
+    let path_secret =
+      match path_secret with
+      | None -> None
+      | Some path_secret -> Some ({path_secret} <: path_secret_nt bytes)
+    in
     let group_secrets = {
       joiner_secret = joiner_secret;
       path_secret = path_secret;
@@ -383,19 +153,30 @@ let rec encrypt_group_secrets #bytes #cb encrypted_group_info joiner_secret key_
 #push-options "--fuel 1"
 val encrypt_welcome:
   #bytes:Type0 -> {|crypto_bytes bytes|} ->
-  welcome_group_info bytes -> bytes -> key_packages:list (key_package_nt bytes tkt & option bytes) -> randomness bytes (encrypt_welcome_entropy_length key_packages) ->
-  result (welcome bytes)
+  group_info_nt bytes -> mls_bytes bytes -> key_packages:list (key_package_nt bytes tkt & option (mls_bytes bytes)) -> randomness bytes (encrypt_welcome_entropy_length key_packages) ->
+  result (welcome_nt bytes)
 let encrypt_welcome #bytes #cb group_info joiner_secret key_packages rand =
   let? encrypted_group_info = (
-    let? welcome_secret = secret_joiner_to_welcome joiner_secret None (*TODO psk*) in
+    let? welcome_secret = secret_joiner_to_welcome #bytes joiner_secret None (*TODO psk*) in
     let? welcome_key = welcome_secret_to_key #bytes welcome_secret in
     let? welcome_nonce = welcome_secret_to_nonce welcome_secret in
-    let? group_info_network = welcome_group_info_to_network group_info in
-    let group_info_bytes = serialize (group_info_nt bytes) group_info_network in
-    aead_encrypt welcome_key welcome_nonce empty group_info_bytes
+    let group_info_bytes = serialize (group_info_nt bytes) group_info in
+    let? encrypted_welcome_group_info = aead_encrypt welcome_key welcome_nonce empty group_info_bytes in
+    if not (length encrypted_welcome_group_info < pow2 30) then
+      error "encrypt_welcome: encrypted_welcome_group_info too long"
+    else
+      return (encrypted_welcome_group_info <: mls_bytes bytes)
   ) in
-  let? group_secrets = encrypt_group_secrets encrypted_group_info joiner_secret key_packages [] (*TODO psks*) rand in
+  let? group_secrets = (
+    let? group_secrets = encrypt_group_secrets encrypted_group_info joiner_secret key_packages [] (*TODO psks*) rand in
+    if not (bytes_length ps_encrypted_group_secrets_nt group_secrets < pow2 30) then
+      error "encrypt_welcome: secrets too long"
+    else
+      return (group_secrets <: mls_list bytes ps_encrypted_group_secrets_nt)
+  ) in
+  let cipher_suite = available_ciphersuite_to_network (ciphersuite #bytes) in
   return ({
+    cipher_suite;
     secrets = group_secrets;
     encrypted_group_info = encrypted_group_info;
   })
@@ -405,28 +186,29 @@ let encrypt_welcome #bytes #cb group_info joiner_secret key_packages rand =
 
 val sign_welcome_group_info:
   #bytes:Type0 -> {|crypto_bytes bytes|} ->
-  sign_private_key bytes -> welcome_group_info bytes -> sign_nonce bytes ->
-  result (welcome_group_info bytes)
+  sign_private_key bytes -> group_info_nt bytes -> sign_nonce bytes ->
+  result (group_info_nt bytes)
 let sign_welcome_group_info #bytes #cb sign_sk gi rand =
-  let? gi_network = welcome_group_info_to_network gi in
-  let tbs_bytes: bytes = serialize (group_info_tbs_nt bytes) gi_network.tbs in
+  let tbs_bytes: bytes = serialize (group_info_tbs_nt bytes) gi.tbs in
   if not (length tbs_bytes < pow2 30 && sign_with_label_pre #bytes "GroupInfoTBS" (length #bytes tbs_bytes)) then error "sign_welcome_group_info: tbs too long"
   else (
     let signature = sign_with_label sign_sk "GroupInfoTBS" tbs_bytes rand in
-    return ({gi with signature = signature})
+    if not (length #bytes signature < pow2 30) then
+      error "sign_welcome_group_info: signature too long"
+    else
+      return ({gi with signature = signature})
   )
 
 val verify_welcome_group_info:
   #bytes:Type0 -> {|crypto_bytes bytes|} ->
-  (nat -> result (sign_public_key bytes)) -> welcome_group_info bytes ->
+  (nat -> result (sign_public_key bytes)) -> group_info_nt bytes ->
   result bool
 let verify_welcome_group_info #bytes #cb get_sign_pk gi =
-  if not (length gi.signature = sign_signature_length #bytes) then
+  if not (length #bytes gi.signature = sign_signature_length #bytes) then
     error "verify_welcome_group_info: bad signature size"
   else (
-    let? gi_network = welcome_group_info_to_network gi in
-    let? sign_pk = get_sign_pk gi.signer in
-    let tbs_bytes: bytes = serialize (group_info_tbs_nt bytes) gi_network.tbs in
+    let? sign_pk = get_sign_pk gi.tbs.signer in
+    let tbs_bytes: bytes = serialize (group_info_tbs_nt bytes) gi.tbs in
     if not (length tbs_bytes < pow2 30 && sign_with_label_pre #bytes "GroupInfoTBS" (length #bytes tbs_bytes)) then error "sign_welcome_group_info: tbs too long"
     else return (verify_with_label sign_pk "GroupInfoTBS" tbs_bytes gi.signature)
   )
